backend/PrintAsm.ml
@@ -103,9 +103,10 @@ module Printer(Target:TARGET) =
 
     let print_globdef oc (name,gdef) =
       match gdef with
-      | Gfun (Internal code) -> print_function oc name code
-      | Gfun (External ef) ->   ()
-      | Gvar v -> print_var oc name v
+      | Some(Gfun (Internal code)) -> print_function oc name code
+      | Some(Gfun (External ef)) ->   ()
+      | Some(Gvar v) -> print_var oc name v
+      | None -> ()
 
     module DwarfTarget: DwarfTypes.DWARF_TARGET =
       struct
