cfrontend/C2C.ml
@@ -294,8 +294,8 @@ let global_for_string s id =
     init := AST.Init_int8(Z.of_uint(Char.code c)) :: !init in
   add_char '\000';
   for i = String.length s - 1 downto 0 do add_char s.[i] done;
-  (id, Gvar {gvar_info = typeStringLiteral s; gvar_init = !init;
-             gvar_readonly = true; gvar_volatile = false})
+  (id, Some(Gvar {gvar_info = typeStringLiteral s; gvar_init = !init;
+             gvar_readonly = true; gvar_volatile = false}))
 
 let name_for_wide_string_literal s =
   try
@@ -335,8 +335,8 @@ let global_for_wide_string s id =
     init := init_of_char(Z.of_uint64 c) :: !init in
   List.iter add_char s;
   add_char 0L;
-  (id, Gvar {gvar_info = typeWideStringLiteral s; gvar_init = List.rev !init;
-             gvar_readonly = true; gvar_volatile = false})
+  (id, Some(Gvar {gvar_info = typeWideStringLiteral s; gvar_init = List.rev !init;
+             gvar_readonly = true; gvar_volatile = false}))
 
 let globals_for_strings globs =
   let globs1 =
@@ -1078,12 +1078,12 @@ let convertFundef loc env fd =
       a_access = Sections.Access_default;
       a_inline = fd.fd_inline && not fd.fd_vararg;  (* PR#15 *)
       a_loc = loc };
-  (id', Gfun(Ctypes.Internal
+  (id', Some(Gfun(Ctypes.Internal
           {fn_return = ret;
            fn_callconv = convertCallconv fd.fd_vararg false fd.fd_attrib;
            fn_params = params;
            fn_vars = vars;
-           fn_body = body'}))
+           fn_body = body'})))
 
 (** External function declaration *)
 
@@ -1106,7 +1106,7 @@ let convertFundecl env (sto, id, ty, optinit) =
     && List.mem_assoc id.name builtins.functions
     then EF_builtin(id'', sg)
     else EF_external(id'', sg) in
-  (id', Gfun(Ctypes.External(ef, args, res, cconv)))
+  (id', Some(Gfun(Ctypes.External(ef, args, res, cconv))))
 
 (** Initializers *)
 
@@ -1166,8 +1166,8 @@ let convertGlobvar loc env (sto, id, ty, optinit) =
       a_loc = loc };
   let volatile = List.mem C.AVolatile attr in
   let readonly = List.mem C.AConst attr && not volatile in
-  (id', Gvar {gvar_info = ty'; gvar_init = init';
-              gvar_readonly = readonly; gvar_volatile = volatile})
+  (id', Some (Gvar {gvar_info = ty'; gvar_init = init';
+              gvar_readonly = readonly; gvar_volatile = volatile}))
 
 (** Convert a list of global declarations.
   Result is a list of CompCert C global declarations (functions +
