cfrontend/PrintCsyntax.ml
@@ -503,8 +503,9 @@ let print_globvar p id v =
 
 let print_globdef p (id, gd) =
   match gd with
-  | Gfun f -> print_fundef p id f
-  | Gvar v -> print_globvar p id v
+  | Some(Gfun f) -> print_fundef p id f
+  | Some(Gvar v) -> print_globvar p id v
+  | None -> ()
 
 let struct_or_union = function Struct -> "struct" | Union -> "union"
 
