backend/Inlining.v
@@ -29,9 +29,9 @@ Definition size_fenv (fenv: funenv) := PTree_Properties.cardinal fenv.
 
 Parameter should_inline: ident -> function -> bool.
 
-Definition add_globdef (fenv: funenv) (idg: ident * globdef fundef unit) : funenv :=
+Definition add_globdef (fenv: funenv) (idg: ident * option (globdef fundef unit)) : funenv :=
   match idg with
-  | (id, Gfun (Internal f)) =>
+  | (id, Some (Gfun (Internal f))) =>
       if should_inline id f
       then PTree.set id f fenv
       else PTree.remove id fenv
